Cslib/Computability/LambdaCalculus/LocallyNameless/Untyped/FullBetaConfluence.lean
@@ -18,14 +18,16 @@ variable {Var : Type u}
 namespace LambdaCalculus.LocallyNameless.Term
 
 /-- A parallel β-reduction step. -/
-@[aesop safe (rule_sets := [LambdaCalculus.LocallyNameless.ruleSet]) [constructors], reduction_sys paraRs "ₚ"]
+@[aesop safe (rule_sets := [LambdaCalculus.LocallyNameless.ruleSet]) [constructors],
+  reduction_sys paraRs "ₚ"]
 inductive Parallel : Term Var → Term Var → Prop
 /-- Free variables parallel step to themselves. -/
 | fvar (x : Var) : Parallel (fvar x) (fvar x)
 /-- A parallel left and right congruence rule for application. -/
 | app : Parallel L L' → Parallel M M' → Parallel (app L M) (app L' M')
 /-- Congruence rule for lambda terms. -/
-| abs (xs : Finset Var) : (∀ x ∉ xs, Parallel (m ^ fvar x) (m' ^ fvar x)) → Parallel (abs m) (abs m')
+| abs (xs : Finset Var) : 
+    (∀ x ∉ xs, Parallel (m ^ fvar x) (m' ^ fvar x)) → Parallel (abs m) (abs m')
 /-- A parallel β-reduction. -/
 | beta (xs : Finset Var) : 
     (∀ x ∉ xs, Parallel (m ^ fvar x) (m' ^ fvar x) ) →
@@ -45,6 +47,18 @@ lemma para_lc_l (step : M ⭢ₚ N) : LC M  := by
   case beta => refine LC.app (LC.abs ?_ _ ?_) ?_ <;> assumption
   all_goals constructor <;> assumption
 
+/-- Parallel reduction is reflexive for locally closed terms. -/
+@[aesop safe (rule_sets := [LambdaCalculus.LocallyNameless.ruleSet])]
+lemma Parallel.lc_refl (M : Term Var) (lc : LC M) : M ⭢ₚ M := by
+  induction lc
+  all_goals constructor <;> assumption
+
+-- TODO: better ways to handle this?
+-- The problem is that sometimes when we apply a theorem we get out of our notation, so aesop can't
+-- see they are the same, including constructors.
+@[aesop safe (rule_sets := [LambdaCalculus.LocallyNameless.ruleSet])]
+lemma Parallel.lc_refl' (M : Term Var) : LC M → Parallel M M := Parallel.lc_refl M
+
 variable [HasFresh Var] [DecidableEq Var]
 
 /-- The right side of a parallel reduction is locally closed. -/
@@ -55,22 +69,9 @@ lemma para_lc_r (step : M ⭢ₚ N) : LC N := by
   case beta => refine beta_lc (LC.abs ?_ _ ?_) ?_ <;> assumption
   all_goals constructor <;> assumption
 
-/-- Parallel reduction is reflexive for locally closed terms. -/
-@[aesop safe (rule_sets := [LambdaCalculus.LocallyNameless.ruleSet])]
-def Parallel.lc_refl (M : Term Var) : LC M → M ⭢ₚ M := by
-  intros lc
-  induction lc
-  all_goals constructor <;> assumption
-
--- TODO: better ways to handle this?
--- The problem is that sometimes when we apply a theorem we get out of our notation, so aesop can't
--- see they are the same, including constructors.
-@[aesop safe (rule_sets := [LambdaCalculus.LocallyNameless.ruleSet])]
-def Parallel.lc_refl' (M : Term Var) : LC M → Parallel M M := Parallel.lc_refl M
-
 omit [HasFresh Var] [DecidableEq Var] in
 /-- A single β-reduction implies a single parallel reduction. -/
-lemma step_to_para (step : M ⭢βᶠ N) : (M ⭢ₚ N) := by
+lemma step_to_para (step : M ⭢βᶠ N) : M ⭢ₚ N := by
   induction step <;> simp only [para_rs_Red_eq]
   case beta _ abs_lc _ => cases abs_lc with | abs xs _ => 
     apply Parallel.beta xs <;> intros <;> apply Parallel.lc_refl <;> aesop
@@ -78,12 +79,12 @@ lemma step_to_para (step : M ⭢βᶠ N) : (M ⭢ₚ N) := by
 
 open FullBeta in
 /-- A single parallel reduction implies a multiple β-reduction. -/
-lemma para_to_redex (para : M ⭢ₚ N) : (M ↠βᶠ N) := by
+lemma para_to_redex (para : M ⭢ₚ N) : M ↠βᶠ N := by
   induction para
   case fvar => constructor
   case app _ _ _ _ l_para m_para redex_l redex_m =>
     trans
-    exact redex_app_l_cong redex_l (para_lc_l m_para)
+    · exact redex_app_l_cong redex_l (para_lc_l m_para)
     exact redex_app_r_cong redex_m (para_lc_r l_para)
   case abs t t' xs _ ih =>
     apply redex_abs_cong xs
@@ -95,71 +96,62 @@ lemma para_to_redex (para : M ⭢ₚ N) : (M ↠βᶠ N) := by
       intros _ mem
       exact para_lc_r (para_ih _ mem)
     calc
-      m.abs.app n ↠βᶠ m'.abs.app n  := redex_app_l_cong (redex_abs_cong xs (λ _ mem ↦ redex_ih _ mem)) (para_lc_l para_n)
+      m.abs.app n ↠βᶠ 
+      m'.abs.app n := 
+        redex_app_l_cong (redex_abs_cong xs (fun _ mem ↦ redex_ih _ mem)) (para_lc_l para_n)
       _           ↠βᶠ m'.abs.app n' := redex_app_r_cong redex_n m'_abs_lc
       _           ⭢βᶠ m' ^ n'       := beta m'_abs_lc (para_lc_r para_n)
 
 /-- Multiple parallel reduction is equivalent to multiple β-reduction. -/
-theorem parachain_iff_redex : (M ↠ₚ N) ↔ (M ↠βᶠ N) := by
-  refine Iff.intro ?chain_to_redex ?redex_to_chain <;> intros h <;> induction' h <;> try rfl
-  case redex_to_chain.tail redex chain => exact Relation.ReflTransGen.tail chain (step_to_para redex)
-  case chain_to_redex.tail para  redex => exact Relation.ReflTransGen.trans redex (para_to_redex para)
+theorem parachain_iff_redex : M ↠ₚ N ↔ M ↠βᶠ N := by
+  refine Iff.intro ?chain_redex ?redex_chain <;> intros h <;> induction' h <;> try rfl
+  case redex_chain.tail redex chain => exact Relation.ReflTransGen.tail chain (step_to_para redex)
+  case chain_redex.tail para  redex => exact Relation.ReflTransGen.trans redex (para_to_redex para)
 
 /-- Parallel reduction respects substitution. -/
-lemma para_subst (x : Var) : (M ⭢ₚ M') → (N ⭢ₚ N') → (M[x := N] ⭢ₚ M'[x := N']) := by
-  intros pm pn
+lemma para_subst (x : Var) (pm : M ⭢ₚ M') (pn : N ⭢ₚ N') : M[x := N] ⭢ₚ M'[x := N'] := by
   induction pm
   case fvar => aesop
   case beta _ _ _ _ xs _ _ ih _ => 
     simp only [open']
     rw [subst_open _ _ _ _ _ (para_lc_r pn)]
-    apply Parallel.beta (xs ∪ {x})
-    intros y ymem
-    simp only [Finset.mem_union, Finset.mem_singleton, not_or] at ymem
-    push_neg at ymem
-    rw [
-      subst_def, 
-      subst_open_var _ _ _ _ _ (para_lc_r pn), 
-      subst_open_var _ _ _ _ _ (para_lc_l pn)
-    ]
-    apply ih
-    all_goals aesop
+    refine Parallel.beta (xs ∪ {x}) ?_ (by assumption)
+    · intros y ymem
+      simp only [Finset.mem_union, Finset.mem_singleton, not_or] at ymem
+      push_neg at ymem
+      rw [
+        subst_def, 
+        subst_open_var _ _ _ _ _ (para_lc_r pn), 
+        subst_open_var _ _ _ _ _ (para_lc_l pn)
+      ] <;> aesop
   case app => constructor <;> assumption
   case abs u u' xs mem ih => 
     apply Parallel.abs (xs ∪ {x})
     intros y ymem
     simp only [Finset.mem_union, Finset.mem_singleton, not_or] at ymem
     repeat rw [subst_def]
-    rw [subst_open_var _ _ _ _ ?_ (para_lc_l pn), subst_open_var _ _ _ _ ?_ (para_lc_r pn)]
     push_neg at ymem
-    apply ih
-    all_goals aesop
+    rw [
+      subst_open_var _ _ _ _ ?_ (para_lc_l pn), 
+      subst_open_var _ _ _ _ ?_ (para_lc_r pn)
+    ] <;> aesop
 
 /-- Parallel substitution respects closing and opening. -/
-lemma para_open_close (x y z) : 
-  (M ⭢ₚ M') → 
-  y ∉ (M.fv ∪ M'.fv ∪ {x}) → 
-  M⟦z ↜ x⟧⟦z ↝ fvar y⟧ ⭢ₚ M'⟦z ↜ x⟧⟦z ↝ fvar y⟧ 
-  := by
-  intros para vars
-  simp only [Finset.union_assoc, Finset.mem_union, Finset.mem_singleton, not_or] at vars
-  rw [open_close_to_subst, open_close_to_subst] 
-  apply para_subst
-  exact para
+lemma para_open_close (x y z) (para : M ⭢ₚ M') (_ : y ∉ M.fv ∪ M'.fv ∪ {x}) :
+    M⟦z ↜ x⟧⟦z ↝ fvar y⟧ ⭢ₚ M'⟦z ↜ x⟧⟦z ↝ fvar y⟧ := by
+  simp only [Finset.union_assoc, Finset.mem_union, Finset.mem_singleton, not_or] at *
+  rw [open_close_to_subst _ _ _ _ (para_lc_l para), open_close_to_subst _ _ _ _ (para_lc_r para)]
+  apply para_subst _ para
   constructor
-  exact para_lc_r para
-  exact para_lc_l para
 
 /-- Parallel substitution respects fresh opening. -/
-lemma para_open_out (L : Finset Var) :
-    (∀ x, x ∉ L → (M ^ fvar x) ⭢ₚ (N ^ fvar x))
-    → (M' ⭢ₚ N') → (M ^ M') ⭢ₚ (N ^ N') := by
-    intros mem para
-    let ⟨x, qx⟩ := fresh_exists (L ∪ N.fv ∪ M.fv)
-    simp only [Finset.union_assoc, Finset.mem_union, not_or] at qx
-    obtain ⟨q1, q2, q3⟩ := qx
-    rw [subst_intro x M' _ q3 (para_lc_l para), subst_intro x N' _ q2 (para_lc_r para)]
-    exact para_subst x (mem x q1) para
+lemma para_open_out (L : Finset Var) (mem : ∀ x, x ∉ L → (M ^ fvar x) ⭢ₚ N ^ fvar x)
+    (para : M' ⭢ₚ N') : (M ^ M') ⭢ₚ (N ^ N') := by
+  let ⟨x, qx⟩ := fresh_exists (L ∪ N.fv ∪ M.fv)
+  simp only [Finset.union_assoc, Finset.mem_union, not_or] at qx
+  obtain ⟨q1, q2, q3⟩ := qx
+  rw [subst_intro x M' _ q3 (para_lc_l para), subst_intro x N' _ q2 (para_lc_r para)]
+  exact para_subst x (mem x q1) para
 
 -- TODO: the Takahashi translation would be a much nicer and shorter proof, but I had difficultly
 -- writing it for locally nameless terms.
@@ -202,20 +194,19 @@ theorem para_diamond : Diamond (@Parallel Var) := by
           simp only [open', close]
           rw [close_open _ _ _ (para_lc_r qt''_l)]
           exact para_subst x qt''_l qt'_l
-        · apply Parallel.beta ((s1'' ^ fvar x).fv ∪ t''.fv ∪ {x})
+        · refine Parallel.beta ((s1'' ^ fvar x).fv ∪ t''.fv ∪ {x}) ?_ (by aesop)
           intros y qy
-          rw [←open_close x s1'' 0]
-          apply para_open_close
-          all_goals aesop
+          rw [←open_close x s1'' 0 (by aesop)]
+          apply para_open_close <;> aesop
     case beta u1' u2' xs' mem' s2pu2' => 
       have ⟨x, qx⟩ := fresh_exists (xs ∪ xs' ∪ u1'.fv ∪ s1'.fv ∪ s2'.fv ∪ u2'.fv)
       simp only [Finset.union_assoc, Finset.mem_union, not_or] at qx
       have ⟨q1, q2, q3, q4, q5, q6⟩ := qx
       have ⟨t', qt'_l, qt'_r⟩ := ih2 s2pu2'
       have ⟨t'', qt''_l, qt''_r⟩ := @ih1 x q1 _ (mem' _ q2)
+      refine ⟨t'' [x := t'], ?_⟩
+      have : _ ∧ _ := ⟨para_subst x qt''_l qt'_l, para_subst x qt''_r qt'_r⟩
       rw [subst_intro x u2' u1' _ (para_lc_l qt'_r), subst_intro x s2' s1' _ (para_lc_l qt'_l)]
-      exists t'' [x := t']
-      exact ⟨para_subst x qt''_l qt'_l, para_subst x qt''_r qt'_r⟩
       all_goals aesop
   case app s1 s1' s2 s2' s1ps1' _ ih1 ih2  =>
     cases tpt2
@@ -252,3 +243,5 @@ theorem confluence_beta : Confluence (@FullBeta Var) := by
     exact parachain_iff_redex
   rw [←eq]
   exact @para_confluence Var _ _
+
+end LambdaCalculus.LocallyNameless.Term
