Cslib/Computability/LambdaCalculus/LocallyNameless/Untyped/FullBeta.lean
@@ -45,14 +45,14 @@ lemma step_lc_l (step : M ⭢βᶠ M') : LC M := by
   induction step <;> constructor
   all_goals assumption
 
-/-- Left congruence rule for application in multiple reduction.-/
+/-- Left congruence rule for application in multiple reduction. -/
 theorem redex_app_l_cong : (M ↠βᶠ M') → LC N → (app M N ↠βᶠ app M' N) := by
   intros redex lc_N 
   induction' redex
   case refl => rfl
   case tail ih r => exact Relation.ReflTransGen.tail r (appR lc_N ih)
 
-/-- Right congruence rule for application in multiple reduction.-/
+/-- Right congruence rule for application in multiple reduction. -/
 theorem redex_app_r_cong : (M ↠βᶠ M') → LC N → (app N M ↠βᶠ app N M') := by
   intros redex lc_N 
   induction' redex
@@ -68,7 +68,8 @@ lemma step_lc_r (step : M ⭢βᶠ M') : LC M' := by
   all_goals try constructor <;> assumption 
 
 /-- Substitution respects a single reduction step. -/
-lemma redex_subst_cong (s s' : Term Var) (x y : Var) : (s ⭢βᶠ s') → (s [ x := fvar y ]) ⭢βᶠ (s' [ x := fvar y ]) := by
+lemma redex_subst_cong (s s' : Term Var) (x y : Var) : 
+    s ⭢βᶠ s' → s [ x := fvar y ] ⭢βᶠ s' [ x := fvar y ] := by
   intros step
   induction step
   case appL ih => exact appL (subst_lc (by assumption) (by constructor)) ih 
@@ -89,7 +90,6 @@ lemma redex_subst_cong (s s' : Term Var) (x y : Var) : (s ⭢βᶠ s') → (s [ 
       subst_fresh x (fvar z) (fvar y), ←subst_fresh x (fvar z) (fvar y),
       ←subst_open x (fvar y) 0 (fvar z) m' (by constructor), subst_fresh x (fvar z) (fvar y)
     ]
-    apply ih
     all_goals aesop
 
 /-- Abstracting then closing preserves a single reduction. -/
@@ -99,9 +99,9 @@ lemma step_abs_close {x : Var} : (M ⭢βᶠ M') → (M⟦0 ↜ x⟧.abs ⭢β�
   intros y _
   simp only [open']
   repeat rw [open_close_to_subst]
-  exact redex_subst_cong M M' x y step
-  exact step_lc_r step
-  exact step_lc_l step
+  · exact redex_subst_cong M M' x y step
+  · exact step_lc_r step
+  · exact step_lc_l step
 
 /-- Abstracting then closing preserves multiple reductions. -/
 lemma redex_abs_close {x : Var} : (M ↠βᶠ M') → (M⟦0 ↜ x⟧.abs ↠βᶠ M'⟦0 ↜ x⟧.abs) :=  by
@@ -109,14 +109,17 @@ lemma redex_abs_close {x : Var} : (M ↠βᶠ M') → (M⟦0 ↜ x⟧.abs ↠β�
   induction step using Relation.ReflTransGen.trans_induction_on
   case ih₁ => rfl
   case ih₂ ih => exact Relation.ReflTransGen.single (step_abs_close ih)
-  case ih₃ l r => trans; exact l; exact r
+  case ih₃ l r => exact .trans l r
 
 /-- Multiple reduction of opening implies multiple reduction of abstraction. -/
-theorem redex_abs_cong (xs : Finset Var) : (∀ x ∉ xs, (M ^ fvar x) ↠βᶠ (M' ^ fvar x)) → M.abs ↠βᶠ M'.abs := by
+theorem redex_abs_cong (xs : Finset Var) : 
+    (∀ x ∉ xs, (M ^ fvar x) ↠βᶠ (M' ^ fvar x)) → M.abs ↠βᶠ M'.abs := by
   intros mem
   have ⟨fresh, union⟩ := fresh_exists (xs ∪ M.fv ∪ M'.fv)
   simp only [Finset.union_assoc, Finset.mem_union, not_or] at union
   obtain ⟨_, _, _⟩ := union
   rw [←open_close fresh M 0 ?_, ←open_close fresh M' 0 ?_]
-  refine redex_abs_close (mem fresh ?_)
+  · exact redex_abs_close (mem fresh (by assumption))
   all_goals assumption
+
+end LambdaCalculus.LocallyNameless.Term.FullBeta
